Ex.Intro: minor progress

state/Examples.Intro.fst
@@ -9,12 +9,19 @@ open FStar.Tactics.Typeclasses
 open SharedRefs
 open Witnessable
 
+let lemma_modifies_only_shared_and_encapsulated h0 h1 #a #rel (r : mref a rel) :
+  Lemma
+    (requires modifies_only_shared_and_encapsulated h0 h1 /\ h0 `contains` r /\ ~(compare_addrs r map_shared) /\ ~(is_shared r h0 \/ is_encapsulated r h0))
+    (ensures sel h0 r == sel h1 r)
+= ()
+
 type callback =
   unit -> SST unit (fun _ -> True) (fun h0 _ h1 -> modifies_only_shared_and_encapsulated h0 h1 /\ gets_shared Set.empty h0 h1)
 
 type lib_type =
   r:ref (ref int) -> SST callback (fun _ -> witnessed (contains_pred r) /\ witnessed (is_shared r)) (fun h0 _ h1 -> modifies_only_shared_and_encapsulated h0 h1 /\ gets_shared Set.empty h0 h1)
 
+// #push-options "--split_queries always"
 let prog (lib : lib_type) : SST unit (requires fun h0 -> True) (ensures fun h0 _ h1 -> True) =
   let secret : ref int = sst_alloc 42 in
   // let h = get_heap () in
@@ -35,5 +42,16 @@ let prog (lib : lib_type) : SST unit (requires fun h0 -> True) (ensures fun h0 _
   // let h = get_heap () in
   sst_write_shareable #(SRef SNat) r v;
   assert (!secret == 42);
+  let h0 = get_heap () in
+  assert (sel h0 secret == 42) ;
   cb ();
-  assume (!secret == 42)
+  let h1 = get_heap () in
+  assert (modifies_only_shared_and_encapsulated h0 h1);
+  assume (~ (is_shared secret h0)) ;
+  assert (h0 `contains` secret);
+  assert (~(compare_addrs secret map_shared));
+  // lemma_modifies_only_shared_and_encapsulated h0 h1 secret ;
+  assume (sel h0 secret == sel h1 secret);
+  // assert (sel h1 secret == 42) ;
+  assert (!secret == 42)
+// #pop-options
